src/program_proof/rsm/distx_tuple.v
@@ -22,8 +22,15 @@ Section program.
     Persistent (is_tuple tuple key α).
   Admitted.
 
+  (* NB: If we were simply to use Paxos rather than PCR, a better way would be
+  requiring the [tid = tsprep], and moving the the length precondition into the
+  tuple invariant. With PCR, however, a tuple could be modified by a txn with a
+  timestamp different from the prepared timestamp. A more fundamental reason to
+  this difference is that while Paxos allows deducing commit safety at the
+  *replica* level, PCR can only deduce such at the *replica group* level. *)
   Theorem wp_Tuple__AppendVersion
     (tuple : loc) (tid : u64) (val : string) key hist tsprep α :
+    (length hist ≤ uint.nat tid)%nat ->
     is_tuple tuple key α -∗
     {{{ tuple_phys_half α key hist tsprep }}}
       Tuple__AppendVersion #tuple #tid #(LitString val)
@@ -61,6 +68,7 @@ Section program.
   Admitted.
 
   Theorem wp_Tuple__KillVersion (tuple : loc) (tid : u64) key hist tsprep α :
+    (length hist ≤ uint.nat tid)%nat ->
     is_tuple tuple key α -∗
     {{{ tuple_phys_half α key hist tsprep }}}
       Tuple__KillVersion #tuple #tid
